theory/System/EquivProofs.v
@@ -7,6 +7,7 @@ Require Import POram.Utils.Classes.
 Import MonadNotation.
 Require Import POram.System.PathORAMFunCorrect.
 Require Import POram.System.Equiv.
+Require Import POram.Utils.StateT.
 
 Section EquivProofs.
 
@@ -31,13 +32,764 @@ Definition read id : Poram nat :=
 Definition write id v : Poram nat :=
   map snd (write_access id v).
 
+Definition triv {X} : X -> Prop :=
+  fun _ => True.
+
+Lemma kv_rel_read_1 : forall k v k',
+  state_plift
+    (fun st => well_formed st /\ kv_rel k v st)
+    (fun st => well_formed st /\ kv_rel k v st)
+    triv
+    (read_access k').
+Proof.
+Admitted.
+
+Lemma kv_rel_read_2 : forall s k v k',
+  plift
+    (fun x => kv_rel k v (snd x) -> kv_rel k v s)
+    (read_access k' s).
+Proof.
+Admitted.
+
+Lemma kv_rel_write_neq : forall k v k' v',
+  k <> k' ->
+  state_plift
+    (fun st => well_formed st /\ kv_rel k v st)
+    (fun st => well_formed st /\ kv_rel k v st)
+    triv
+    (write_access k' v').
+Proof.
+Admitted.
+
+Lemma kv_rel_write_eq : forall k v,
+  state_plift
+    well_formed
+    (fun st => well_formed st /\ kv_rel k v st)
+    triv
+    (write_access k v).
+Proof.
+Admitted.
+
+Definition state_plift2 {M} `{PredLift2 M} {S X Y}
+  (Pre Post : S -> S -> Prop)
+  (P : X -> Y -> Prop)
+  (m1 : StateT S M X)
+  (m2 : StateT S M Y) : Prop :=
+  forall s1 s2,
+    Pre s1 s2 ->
+    plift2 (prod_rel P Post) (m1 s1) (m2 s2).
+
+Lemma state_plift2_ret {M} `{PredLift M} {S X Y}
+  (Pre : S -> S -> Prop)
+  (P : X -> Y -> Prop) : forall x y,
+  P x y -> state_plift2 Pre Pre P
+    (mreturn x) (mreturn y).
+Proof.
+  intros x y Hxy s1 s2 Hs1s2.
+  apply plift2_ret.
+  split; auto.
+Qed.
+
+Lemma state_plift2_bind {M} `{PredLift2 M}
+  {S X Y X' Y'}
+  (Pre Mid Post : S -> S -> Prop)
+  (P : X -> Y -> Prop)
+  (Q : X' -> Y' -> Prop)
+  (m1 : StateT S M X)
+  (m2 : StateT S M Y)
+  (f1 : X -> StateT S M X')
+  (f2 : Y -> StateT S M Y') :
+  state_plift2 Pre Mid P m1 m2 ->
+  (forall x y, P x y ->
+    state_plift2 Mid Post Q (f1 x) (f2 y)) ->
+  state_plift2 Pre Post Q
+    (mbind m1 f1) (mbind m2 f2).
+Proof.
+  intros Hm1m2 Hf1f2 s1 s2 Hs1s2.
+  eapply plift2_bind.
+  - apply Hm1m2; auto.
+  - intros [x s] [y s'] [H1 H2]; simpl in *.
+    apply Hf1f2; auto.
+Qed.
+
+Definition equiv {X} (m1 m2 : Poram X) : Prop :=
+  state_plift2
+    (fun s1 s2 =>
+      well_formed s1 /\
+      well_formed s2 /\
+      state_equiv s1 s2)
+    (fun s1 s2 =>
+      well_formed s1 /\
+      well_formed s2 /\
+      state_equiv s1 s2)
+    eq m1 m2.
+
+Lemma equiv_implies_poram_equiv {X}
+  (m1 m2 : Poram X) :
+  equiv m1 m2 ->
+  poram_equiv eq m1 m2.
+Proof.
+  intros eqv s1 s2 Hs1s2 wf_s1 wf_s2.
+  pose proof (conj wf_s1 (conj wf_s2 Hs1s2)) as pf.
+  specialize (eqv s1 s2 pf).
+  destruct (m1 s1), (m2 s2); simpl in *.
+  eapply Forall_impl; [|exact eqv].
+  intros [x s] Hxs.
+  eapply Forall_impl; [|exact Hxs].
+  intros [x' s'] [H1 [H2 [H3 H4]]].
+  split; auto.
+Qed.
+
+Definition triv2 {X Y} : X -> Y -> Prop :=
+  fun _ _ => True.
+
+Definition lawful {M} `{PredLift2 M} {S X}
+  (m : StateT S M X) (Pre : S -> S -> Prop) :=
+  state_plift2 Pre Pre eq m m.
+
+Definition pand {X} (P Q : X -> Prop) : X -> Prop :=
+  fun x => P x /\ Q x.
+
+Lemma write_access_wf2_eq : forall
+  (id : block_id) (v_old v_new : nat),
+  state_plift
+  (pand well_formed (kv_rel id v_old))
+  (pand well_formed (kv_rel id v_new))
+  (has_value v_old)
+  (write_access id v_new).
+Proof.
+Admitted.
+
+Lemma write_access_wf2_neq : forall
+  (id id' : block_id) (v v' : nat),
+  id <> id' ->
+  state_plift
+  (pand well_formed (kv_rel id' v'))
+  (pand well_formed (kv_rel id' v'))
+  (has_value v)
+  (write_access id v).
+Proof.
+Admitted.
+
+Lemma state_plift2_write_write k v : 
+  state_plift2
+  (fun s1 s2 : state =>
+    well_formed s1 /\
+    well_formed s2 /\
+    state_equiv s1 s2)
+  (fun s1 s2 : state =>
+    well_formed s1 /\
+    well_formed s2 /\
+    state_equiv s1 s2 /\
+    kv_rel k v s1)
+  triv2
+  (write k v)
+  (write k v).
+Proof.
+  intros s s'.
+  intros [H1 [H2 H3]].
+  unfold plift2.
+  unfold Pred_Dist_Lift2.
+  unfold dist_lift2.
+  eapply plift_bind.
+  - eapply write_access_wf; auto.
+  - intros [] pfs.
+    apply plift_ret.
+    eapply plift_bind.
+    + eapply write_access_wf2_eq.
+      split; auto.
+      admit.
+    + intros [] pfs2.
+      apply plift_ret.
+      simpl; split.
+      * exact I.
+      * simpl.
+        split; try tauto.
+        split; try tauto.
+        admit.
+        split.
+        split; try tauto.
+
+
+(* TODO: make write_access_wf_2 like read_access_wf_2 *)
+Admitted.
+
+Definition pforall {I X} (P : I -> X -> Prop) : X -> Prop :=
+  fun x => forall i, P i x.
+
+Lemma plift_conj {M} `{PredLift M} {X}
+  (P Q : X -> Prop) (m : M X) :
+  plift P m ->
+  plift Q m ->
+  plift (pand P Q) m.
+Proof.
+Admitted.
+
+Lemma plift_forall {I X}
+  (P : I -> X -> Prop) (m : dist X) :
+  (forall i, plift (P i) m) ->
+  plift (pforall P) m.
+Proof.
+  intros.
+  unfold pforall.
+  unfold plift in *; simpl in *.
+  destruct m as [l q]; simpl in *; clear q.
+  rewrite Forall_forall.
+  intros x Hx i.
+  specialize (H i).
+  rewrite Forall_forall in H.
+  apply H; auto.
+Qed.
+
+Lemma plift2_forall {I X Y}
+  (P : I -> X -> Y -> Prop)
+  (m : dist X) (m' : dist Y) :
+  (forall i, plift2 (P i) m m') ->
+  plift2 (fun x y => forall i, P i x y) m m'.
+Proof.
+  intros.
+  unfold pforall; simpl in *.
+  unfold dist_lift2 in *; simpl in *.
+  unfold dist_lift in *.
+  destruct m as [l q]; simpl in *; clear q.
+  destruct m' as [l' q']; simpl in *; clear q'.
+  rewrite Forall_forall.
+  intros x Hx.
+  rewrite Forall_forall.
+  intros y Hy i.
+  specialize (H i).
+  rewrite Forall_forall in H.
+  specialize (H x Hx).
+  rewrite Forall_forall in H.
+  apply H; auto.
+Qed.
+
+Lemma state_plift_split {M} `{PredLift M} {S X}
+  (m : StateT S M X)
+  (Pre Post1 Post2 : S -> Prop)
+  (P : X -> Prop) :
+  has_weakening M ->
+  state_plift Pre Post1 P m ->
+  state_plift Pre Post2 triv m ->
+  state_plift Pre (pand Post1 Post2) P m.
+Proof.
+  intros.
+  intros s Hs.
+  specialize (H2 s Hs).
+  specialize (H3 s Hs).
+  pose proof (plift_conj _ _ _ H2 H3).
+  eapply H1; [|exact H4].
+  intros [x s'] [[H5 H6] [_ H7]].
+  split; auto.
+  split; auto.
+Qed.
+
+Lemma state_plift_proj1 {M} `{PredLift M} {S X}
+  (m : StateT S M X)
+  (Pre1 Pre2 Post : S -> Prop)
+  (P : X -> Prop) :
+  state_plift Pre1 Post P m ->
+  state_plift (pand Pre1 Pre2) Post P m.
+Proof.
+  intros Hm s [Hs _].
+  apply (Hm s Hs).
+Qed.
+
+Lemma kv_rel_functional : forall s,
+  well_formed s ->
+  forall k v v',
+    kv_rel k v s ->
+    kv_rel k v' s ->
+    v = v'.
+Proof.
+Admitted.
+
+Lemma impl_dist {X} (m : dist X)
+  (P : Prop) (Q : X -> Prop) :
+  (P -> plift Q m) ->
+  plift (fun x => P -> Q x) m.
+Proof.
+  intro.
+  unfold plift in *.
+  simpl in *.
+  destruct m as [l q]; simpl in *; clear q.
+  rewrite Forall_forall in *.
+  firstorder.
+Qed.
+
+Lemma impl_trans {X} (m : dist X)
+  (P Q R : X -> Prop) :
+  plift (fun x => P x -> Q x) m ->
+  plift (fun x => Q x -> R x) m ->
+  plift (fun x => P x -> R x) m.
+Proof.
+  unfold plift; simpl.
+  destruct m as [l q]; simpl; clear q.
+  repeat rewrite Forall_forall.
+  firstorder.
+Qed.
+
+Lemma plift_triv {X} (m : dist X) (P : Prop) :
+  P -> plift (fun _ => P) m.
+Proof.
+  destruct m as [l q].
+  unfold plift; simpl; clear q.
+  rewrite Forall_forall.
+  tauto.
+Qed.
+
+Lemma read_access_wf2 : forall
+  (id : block_id) (v : nat) s,
+  state_plift
+  (pand (pand well_formed (kv_rel id v)) (state_equiv s))
+  (pand (pand well_formed (kv_rel id v)) (state_equiv s))
+  (has_value v)
+  (read_access id).
+Proof.
+  intros id v s'.
+  apply state_plift_split.
+  - apply dist_has_weakening.
+  - apply state_plift_proj1.
+    apply read_access_wf.
+  - intros s [[H1 H2] H3].
+    eapply dist_has_weakening with
+      (P := fun x => state_equiv s' (snd x)).
+    + intros [p s1] H4; split; auto.
+      exact I.
+    + eapply plift_forall.
+      intro id'.
+      eapply plift_forall.
+      intro v'.
+      apply plift_conj.
+      * apply impl_dist.
+        intro.
+        assert (kv_rel id' v' s) by (apply H3; auto).
+        pose proof (kv_rel_read_1 id' v' id s
+          (conj H1 H0)).
+        eapply dist_has_weakening; [|exact H4].
+        intros [] pfs.
+        apply pfs.
+      * apply impl_trans with (Q := fun _ => kv_rel id' v' s).
+        -- apply kv_rel_read_2.
+        -- eapply plift_triv.
+           apply H3.
+Qed.
+
+Lemma state_equiv_sym : forall s s',
+  state_equiv s s' ->
+  state_equiv s' s.
+Admitted.
+
+Definition sigma {X} (P : X -> Prop) (m : dist X) : Prop :=
+  Exists P (List.map fst (dist_pmf m)).
+
+Lemma curry {X} (P : X -> Prop) (Q : Prop) (m : dist X) :
+  (sigma P m -> Q) ->
+  plift (fun x => P x -> Q) m.
+Proof.
+  unfold sigma, plift; simpl.
+  unfold dist_lift.
+  destruct m as [l q]; simpl; clear q.
+  intro pf.
+  rewrite Forall_forall.
+  intros x Hx1 Hx2.
+  apply pf.
+  rewrite Exists_exists.
+  exists x; tauto.
+Qed.
+
+Lemma foobar k v :
+  state_plift2
+    (fun s s' =>
+      state_equiv s s' /\
+      kv_rel k v s /\
+      kv_rel k v s')
+    state_equiv
+    (fun x x' => x = v /\ x' = v)
+    (mreturn v)
+    (read k).
+Proof.
+  intros s s' [eq_ss' [kv_s kv_s']].
+  unfold plift2.
+  apply plift_ret.
+  apply plift_conj.
+  - apply plift_conj; simpl fst.
+    + apply plift_triv; reflexivity.
+    + eapply plift_bind.
+      * apply read_access_wf; split.
+        -- admit.
+        -- exact kv_s'.
+      * intros [] ?.
+        apply plift_ret.
+        destruct H.
+        destruct p; simpl.
+        unfold has_value in H.
+        symmetry; exact H.
+  - simpl snd.
+Admitted.
+
+Lemma state_plift2_ret_l {S X} (x : X)
+  (m : StateT S dist X) Pre Post P :
+  (forall s, state_plift (Pre s) (Post s) (P x) m) ->
+  state_plift2 Pre Post P (mreturn x) m.
+Proof.
+  intros Hm s s' HPre.
+  apply plift_ret.
+  unfold state_plift in Hm.
+  specialize (Hm s s' HPre).
+  eapply dist_has_weakening; [|exact Hm].
+  unfold prod_rel.
+  intros []; simpl; tauto.
+Qed.
+
+Axiom cheat : forall {X}, X.
+
+Lemma state_plift2_conj {S X Y}
+  (Pre Post1 Post2 : S -> S -> Prop)
+  (P : X -> Y -> Prop)
+  (m1 : StateT S dist X)
+  (m2 : StateT S dist Y) :
+  state_plift2 Pre Post1 P m1 m2 ->
+  state_plift2 Pre Post2 P m1 m2 ->
+  state_plift2 Pre (fun s s' => Post1 s s' /\ Post2 s s') P m1 m2.
+Proof.
+Admitted.
+
+Lemma state_plift2_forall {S V X Y}
+  (Pre : S -> S -> Prop)
+  (Post : V -> S -> S -> Prop)
+  (P : X -> Y -> Prop)
+  (m1 : StateT S dist X)
+  (m2 : StateT S dist Y) :
+  (forall v, state_plift2 Pre (Post v) P m1 m2) ->
+  state_plift2 Pre (fun s s' => forall v, Post v s s') P m1 m2.
+Proof.
+Admitted.
+
+Lemma split_post_and_pred {S X Y}
+  (m : StateT S dist X)
+  (m' : StateT S dist Y) Pre Post P :
+  state_plift2 Pre triv2 P m m' ->
+  state_plift2 Pre Post triv2 m m' ->
+  state_plift2 Pre Post P m m'.
+Proof.
+  intros H1 H2 s s' eq_ss'.
+  specialize (H1 s s' eq_ss').
+  specialize (H2 s s' eq_ss').
+  unfold plift2 in *; simpl in *.
+  unfold dist_lift2 in *.
+  unfold plift in *; simpl in *.
+  destruct (m s) as [l q].
+  destruct (m' s') as [l' q'].
+  unfold dist_lift in *; simpl in *.
+  clear q q'.
+  rewrite Forall_forall in *.
+  intros p Hp.
+  specialize (H1 p Hp).
+  specialize (H2 p Hp).
+  rewrite Forall_forall in *.
+  intros q Hq.
+  specialize (H1 q Hq).
+  specialize (H2 q Hq).
+  destruct H1 as [H1 _].
+  destruct H2 as [_ H2].
+  split; auto.
+Qed.
+
+Definition undef k s :=
+  ~ exists v, kv_rel k v s.
+
+Lemma def_or_undef k s :
+  { exists v, kv_rel k v s } +
+  { undef k s }.
+Proof.
+Admitted.
+
+Lemma read_pres_kv k v k' :
+  state_plift (kv_rel k v) (kv_rel k v) triv
+  (read k').
+Admitted.
+
+Lemma read_pres_undef k k' :
+  state_plift (undef k) (undef k) triv
+  (read k').
+Admitted.
+
+Lemma function_property : forall s k v v',
+  kv_rel k v s -> kv_rel k v' s -> v = v'.
+Admitted.
+
+Lemma read_val k v :
+  state_plift (kv_rel k v) triv (eq v) (read k).
+Proof.
+Admitted.
+
+Lemma write_val_eq k v :
+  state_plift triv (kv_rel k v) triv (write k v).
+Proof.
+Admitted.
+
+Lemma write_val_neq k v k' v' :
+  k <> k' ->
+  state_plift (kv_rel k' v') (kv_rel k' v') triv (write k v).
+Proof.
+Admitted.
+
+Lemma read_pres_equiv k' s :
+  state_plift (state_equiv s) (state_equiv s) triv (read k').
+Proof.
+  intros s' eq_ss'.
+  eapply dist_has_weakening with
+    (P := fun p => state_equiv s (snd p)).
+  - intros [] pf; split; auto.
+    exact I.
+  - apply plift_forall.
+    intro k.
+    apply plift_forall.
+    intro v.
+    apply plift_conj.
+    + apply impl_dist.
+      intro pf.
+      apply eq_ss' in pf.
+      pose proof (read_pres_kv k v k' s' pf).
+      eapply dist_has_weakening; [|exact H].
+      intros []; tauto.
+    + destruct (def_or_undef k s').
+      * destruct e.
+        pose (read_pres_kv k x k' s' H).
+        eapply dist_has_weakening; [|exact p].
+        intros [] [_ pf] pf'.
+        simpl in pf'.
+        apply eq_ss'.
+        rewrite (function_property _ _ _ _ pf' pf).
+        auto.
+      * pose (read_pres_undef k k' s' u).
+        eapply dist_has_weakening; [|exact p].
+        intros [] [_ pf]; simpl; intros pf'.
+        elim pf.
+        exists v; exact pf'.
+Qed.
+
+Definition dummy {X Y} (P : X -> Prop) (Q : Y -> Prop) : X -> Y -> Prop :=
+  fun x y => P x /\ Q y.
+
+Lemma state_plift2_strengthen_pre {S X Y}
+  (Pre Pre' Post : S -> S -> Prop)
+  (P : X -> Y -> Prop)
+  (m : StateT S dist X)
+  (m' : StateT S dist Y) :
+  (forall s s', Pre' s s' -> Pre s s') ->
+  state_plift2 Pre Post P m m' ->
+  state_plift2 Pre' Post P m m'.
+Proof.
+  intros HPre'Pre H1 s s' Hss'.
+  apply H1.
+  apply HPre'Pre.
+  exact Hss'.
+Qed.
+
+Lemma plift2_conj {X X' Y Y'}
+  (P : X -> Y -> Prop)
+  (Q : X' -> Y' -> Prop)
+  (dx : dist (X * X')) (dy : dist (Y * Y')) :
+  plift2 (fun p p' => P (fst p) (fst p')) dx dy ->
+  plift2 (fun p p' => Q (snd p) (snd p')) dx dy ->
+  plift2 (prod_rel P Q) dx dy.
+Proof.
+  unfold plift2; simpl.
+  unfold dist_lift2.
+  intros.
+  unfold plift in *; simpl in *.
+  destruct dx as [l q]; simpl in *; clear q.
+  rewrite Forall_forall in *.
+  intros p Hp.
+  specialize (H p Hp).
+  specialize (H0 p Hp).
+  unfold dist_lift in *; destruct dy as [l' q'].
+  simpl in *; clear q'.
+  rewrite Forall_forall in *.
+  intros q Hq.
+  split.
+  - apply H; auto.
+  - apply H0; auto.
+Qed.
+
+Lemma plift2_triv {X Y} (dx : dist X) (dy : dist Y)
+  (P : Prop) :
+  P -> plift2 (fun _ _ => P) dx dy.
+Proof.
+  intro.
+  unfold plift2.
+  simpl.
+  unfold dist_lift2.
+  apply plift_triv.
+  apply plift_triv.
+  auto.
+Qed.
+
+Lemma state_plift_split_dummy {S X Y}
+  (Pre Pre' Post Post' : S -> Prop)
+  (m : StateT S dist X) (m' : StateT S dist Y) :
+  state_plift Pre Post triv m ->
+  state_plift Pre' Post' triv m' ->
+  state_plift2 (dummy Pre Pre') (dummy Post Post') triv2 m m'.
+Proof.
+  intros H1 H2 s s' [Hs Hs'].
+  specialize (H1 _ Hs).
+  specialize (H2 _ Hs').
+  apply plift2_conj.
+  - unfold triv2. apply plift2_triv.
+    exact I.
+  - unfold plift2; simpl.
+    unfold dist_lift2.
+    eapply dist_has_weakening; [|exact H1].
+    intros [] [_ pf].
+    eapply dist_has_weakening; [|exact H2].
+    intros [] [_ pf'].
+    split; auto.
+Qed.
+
+Axiom cheat2 : forall {X}, X.
+
+Lemma plift2_and {X Y} {P Q : X -> Y -> Prop}
+  (m : dist X) (m' : dist Y) :
+  plift2 P m m' ->
+  plift2 Q m m' ->
+  plift2 (fun x y => P x y /\ Q x y) m m'.
+Proof.
+Admitted.
+
+Lemma plift2_implication {X Y}
+  {P : X -> Prop} {Q : Y -> Prop}
+  (m : dist X) (m' : dist Y) :
+  (sigma P m -> plift Q m') ->
+  plift2 (fun x y => P x -> Q y) m m'.
+Proof.
+  unfold plift2; simpl.
+  unfold dist_lift2.
+  unfold plift; simpl.
+  unfold dist_lift, sigma.
+  destruct m as [l q]; simpl; clear q.
+  destruct m' as [l' q']; simpl; clear q'.
+  repeat rewrite Forall_forall.
+  rewrite Exists_exists.
+  intro pf.
+  intros x Hx.
+  rewrite Forall_forall.
+  intros y Hy p.
+  apply pf; auto.
+  exists x; split; auto.
+Qed.
+
+Lemma plift2_implication2 {X Y}
+  {P : X -> Prop} {Q : Y -> Prop}
+  (m : dist X) (m' : dist Y) :
+  (sigma Q m' -> plift P m) ->
+  plift2 (fun x y => Q y -> P x) m m'.
+Proof.
+  unfold plift2; simpl.
+  unfold dist_lift2.
+  unfold plift; simpl.
+  unfold dist_lift, sigma.
+  destruct m as [l q]; simpl; clear q.
+  destruct m' as [l' q']; simpl; clear q'.
+  repeat rewrite Forall_forall.
+  rewrite Exists_exists.
+  intro pf.
+  intros x Hx.
+  rewrite Forall_forall.
+  intros y Hy p.
+  apply pf; auto.
+  exists y; split; auto.
+Qed.
+
 Theorem write_read : forall k v,
   poram_equiv
   eq
-  (write k v;; read k) 
-  (write k v;; mreturn v).
+  (write k v;; mreturn v)
+  (write k v;; read k).
 Proof.
+  intros.
+  intros s s'.
+  intros.
+  apply equiv_implies_poram_equiv; auto.
+  unfold equiv.
+  apply split_post_and_pred.
+  - eapply state_plift2_bind with
+      (Mid := dummy (kv_rel k v) (kv_rel k v))
+      (P := triv2).
+    + apply state_plift2_strengthen_pre with
+        (Pre := dummy well_formed well_formed).
+      * unfold dummy; tauto.
+      * apply state_plift_split_dummy.
+        -- intros t _.
+           apply write_val_eq; exact I.
+        -- intros t _.
+           apply write_val_eq; exact I.
+    + intros _ _ _.
+      apply state_plift2_ret_l.
+      intro.
+      pose (read_val k v).
+      intros t [_ Ht].
+      specialize (s1 t Ht).
+      eapply dist_has_weakening; [|exact s1].
+      intros [] [pf _]; split; auto. exact I.
+  - apply state_plift2_bind with
+      (Mid := fun s1 s2 => well_formed s1 /\ well_formed s2 /\ state_equiv s1 s2) (P := triv2).
+    + apply state_plift2_conj.
+      * admit.
+      * apply state_plift2_conj.
+        -- admit.
+        -- intros t t' pfs.
+           unfold plift2; simpl.
+           apply plift2_conj.
+           ++ unfold triv2.
+              apply plift2_triv; auto.
+           ++ apply plift2_forall.
+              intro k'.
+              apply plift2_forall.
+              intro v'.
+              destruct (nat_eq_dec k k').
+              ** subst; apply plift2_and.
+                 --- apply plift2_implication.
+                     intro pf.
+                     assert (v = v').
+                     { admit. }
+                     subst.
+                     epose (write_val_eq k' v' t' I).
+                     eapply dist_has_weakening; [|exact p].
+                     intros []; simpl; tauto.
+                 --- apply plift2_implication2.
+                     intro pf.
+                     assert (v = v').
+                     { admit. }
+                     subst.
+                     epose (write_val_eq k' v' t I).
+                     eapply dist_has_weakening; [|exact p].
+                     intros []; simpl; tauto.
+              ** apply plift2_and.
+                 --- apply plift2_implication.
+                     intro pf.
+                     assert (kv_rel k' v' t').
+                     { admit. }
+                     epose (write_val_neq k v k' v' n t' H2).
+                     eapply dist_has_weakening; [|exact p].
+                     intros []; simpl; tauto.
+                 --- apply plift2_implication2.
+                     intro pf.
+                     assert (kv_rel k' v' t).
+                     { admit. }
+                     epose (write_val_neq k v k' v' n t H2).
+                     eapply dist_has_weakening; [|exact p].
+                     intros []; simpl; tauto.
+    + intros _ _ _.
+      apply state_plift2_ret_l.
+      intro s''. Search state_plift.
+      pose (read_pres_equiv k s'').
+      admit.
 Admitted.
+
+Print Assumptions write_read.
 
 End EquivProofs.
 
